src/search/LinealSearch.dfy
@@ -1,30 +1,23 @@
 
 method LinealSearch(A:array<int>, key:int) returns (index:int)
-    ensures 0 <= index ==> index < A.Length && A[index] == key
-    ensures index < 0 ==> key !in A[..]
+  ensures 0 <= index ==> index < A.Length && A[index] == key
+  ensures index < 0 ==> key !in A[..]
 {
-    var N := A.Length;
-    var i := 0;
-    while i < N
-        invariant 0 <= i <= N
-        // Ningún elemento tal que su índice sea menor al actual puede ser el elemento buscado
-        invariant forall k :: 0 <= k < i ==> A[k] != key
-        decreases N - i
+  var N := A.Length;
+  var i := 0;
+  while i < N
+    invariant 0 <= i <= N
+    // Ningún elemento tal que su índice sea menor al actual puede ser el elemento buscado
+    invariant forall k :: 0 <= k < i ==> A[k] != key
+    decreases N - i
+  {
+    if A[i] == key
     {
-        if A[i] == key
-        {
-            return i;
-        }
-        i := i + 1;
+        return i;
     }
-    return -1;
-}
-
-method Main() {
-    var a := new int[10];
-    a[0], a[1], a[2], a[3], a[4], a[5], a[6], a[7], a[8], a[9] := 2, 4, 6, 8, 10, 12, 14, 16, 18, 20;
-    var index := LinealSearch(a, 12);
-    print index;
+    i := i + 1;
+  }
+  return -1;
 }
 
 /* Explicación:
