src/sort/InsertionSort.dfy
@@ -32,13 +32,6 @@ method InsertionSort(A:array<int>)
   }
 }
 
-method Main() {
-  var A := new int[10];
-  A[0], A[1], A[2], A[3], A[4], A[5], A[6], A[7], A[8], A[9] := 2, 4, 6, 15, 3, 19, 17, 16, 18, 1;
-  InsertionSort(A);
-  print A[..];
-}
-
 /* Explicación:
 
 invariant forall m, n :: 0 <= m < n < i+1 && n != j ==> A[m] <= A[n]
