src/sort/TreeSort.dfy
@@ -1,45 +1,22 @@
 include "../../src/Sorted.dfy"
 include "../data-types/binary-tree/BinaryTree.dfy"
 
-method TreeSort(A:array<int>) returns (sortedSeq:seq<int>)
-    requires A.Length > 0
+method TreeSort(L:List<int>) returns (sorted:List<int>)
+  requires List_Size(L) > 0
 {
-    var N := A.Length;
-    var searchTree := new TreeSet();
+  var N := List_Size(L);
+  var list := L;
+  var tree: BinaryTree<int> := Leaf;
 
-    var i := 0;
-    while i < N
-        invariant 0 <= i <= N
-        decreases N-i
-    {
-        searchTree.insert(A[i]);
-        i := i + 1;
-    }
+  while list != List_Empty
+    decreases list
+  {
+    var head: int := List_Head(list);
+    tree := BinaryTree_Insert(tree, head);
+    list := List_Tail(list);
+  }
 
-    sortedSeq := searchTree.asSeq();
+  sorted := BinaryTree_InOrderElems(tree);
 
-    return sortedSeq;
-}
-
-method Main() {
-    var A := new int[10];
-    A[0], A[1], A[2], A[3], A[4], A[5], A[6], A[7], A[8], A[9] := 2, 4, 6, 8, 10, 12, 14, 16, 18, 20;
-    var searchTree := new TreeSet();
-    searchTree.insert(A[0]);
-    searchTree.insert(A[1]);
-    searchTree.insert(A[2]);
-    searchTree.insert(A[3]);
-    searchTree.insert(A[4]);
-    searchTree.insert(A[5]);
-    searchTree.insert(A[6]);
-    searchTree.insert(A[7]);
-    searchTree.insert(A[8]);
-    searchTree.insert(A[9]);
-    var sortedSeq := searchTree.asSeq();
-    print sortedSeq;
-
-    var B := new int[10];
-    B[0], B[1], B[2], B[3], B[4], B[5], B[6], B[7], B[8], B[9] := 2, 4, 6, 8, 10, 12, 14, 16, 18, 20;
-    var sortedSeqB := TreeSort(B);
-    print sortedSeqB;
+  return sorted;
 }
