test/data-types/list/ListTest.dfy
@@ -3,6 +3,8 @@ include "../../../src/data-types/list/List.dfy"
 method Main() {
   InsertIntoListTest();
   ConcatTwoListsTest();
+  SizeZeroTest();
+  SizeTest();
 }
 
 method InsertIntoListTest() {
@@ -12,20 +14,33 @@ method InsertIntoListTest() {
   list := List_Insert(list, 4);
   list := List_Insert(list, 12);
   list := List_Insert(list, 7);
-
-  assert(list == Cons(2, Cons(10, Cons(4, Cons(12, Cons(7, List_Empty))))));
+  var expected := Cons(2, Cons(10, Cons(4, Cons(12, Cons(7, List_Empty)))));
+  assert(expected == list);
 }
 
 method ConcatTwoListsTest() {
   var a: List<int> := List_Empty;
   a := List_Insert(a, 2);
   a := List_Insert(a, 10);
-
   var b: List<int> := List_Empty;
   b := List_Insert(b, 4);
   b := List_Insert(b, 12);
   b := List_Insert(b, 7);
-
   var c := List_Concat(a, b);
-  assert(c == Cons(2, Cons(10, Cons(4, Cons(12, Cons(7, List_Empty))))));
+  var expected := Cons(2, Cons(10, Cons(4, Cons(12, Cons(7, List_Empty)))));
+  assert(expected == c);
+}
+
+method SizeZeroTest() {
+  var list: List<int> := List_Empty;
+  var size := List_Size(list);
+  var expected := 0;
+  assert(expected == size);
+}
+
+method SizeTest() {
+  var list: List<int> := Cons(2, Cons(10, Cons(4, Cons(12, Cons(7, List_Empty)))));
+  var size := List_Size(list);
+  var expected := 5;
+  assert(expected == size);
 }
