test/search/LinealSearchTest.dfy
@@ -1,0 +1,12 @@
+include "../../src/search/LinealSearch.dfy"
+
+method Main() {
+  LinealSearchTest();
+}
+
+method LinealSearchTest() {
+  var a := new int[10];
+  a[0], a[1], a[2], a[3], a[4], a[5], a[6], a[7], a[8], a[9] := 2, 4, 6, 8, 10, 12, 14, 16, 18, 20;
+  var index := LinealSearch(a, 12);
+  print index;
+}
