test/sort/BubbleSortTest.dfy
@@ -1,0 +1,12 @@
+include "../../src/sort/BubbleSort.dfy"
+
+method Main() {
+  BubbleSortTest();
+}
+
+method BubbleSortTest() {
+  var A := new int[10];
+  A[0], A[1], A[2], A[3], A[4], A[5], A[6], A[7], A[8], A[9] := 2, 4, 6, 15, 3, 19, 17, 16, 18, 1;
+  BubbleSort(A);
+  print A[..];
+}
