test/sort/TreeSortTest.dfy
@@ -1,0 +1,11 @@
+include "../../src/sort/TreeSort.dfy"
+
+method Main() {
+  TreeSortTest();
+}
+
+method TreeSortTest() {
+  var list := Cons(2, Cons(10, Cons(4, Cons(12, Cons(7, List_Empty)))));
+  var sorted := TreeSort(list);
+  List_Print(sorted);
+}
